Switch from LData to DData for consistency

ocaml/src/Asts.mli
@@ -26,7 +26,7 @@ type camp = Compiler.pat
 type algenv = Compiler.algenv
 type nrc = Compiler.nrc
 type dnrc = (Compiler.__, algenv) Compiler.dnrc
-type nrcmr = (Compiler.var * Compiler.localization) list * Compiler.nrcmr
+type nrcmr = (Compiler.var * Compiler.dlocalization) list * Compiler.nrcmr
 type cldmr = Compiler.cld_mrl
 
 type sexp_ast = SExp.sexp
