coq/Compiler/Top/CompBack.v
@@ -46,14 +46,13 @@ Module CompBack(runtime:CompilerRuntime).
 
   (* Compilation from NNRCMR to CloudantMR *)
 
-  Require LData.
-  Definition localization := LData.localization.
+  Definition localization := DData.dlocalization.
 
   Require Import NNRCMR CloudantMR NNRCMRtoCloudant CloudantMRtoJavascript ForeignToCloudant.
   Require Import NRewMR.
 
   (* Java equivalent: MROptimizer.optimize *)
-  Definition nrcmr_to_nrcmr_prepared_for_cldmr (env_vars:list (var * localization)) (e_mr:nrcmr) : nrcmr :=
+  Definition nrcmr_to_nrcmr_prepared_for_cldmr (env_vars:list (var * dlocalization)) (e_mr:nrcmr) : nrcmr :=
     let e_mr := foreign_to_cloudant_prepare_nrcmr e_mr in
     let e_mr := mr_optimize e_mr in
     (* Maybe add call to nnrc_to_nnrcmr_no_chain in case e_mr is more than one Map/Reduce *)
@@ -61,10 +60,10 @@ Module CompBack(runtime:CompilerRuntime).
     let e_mr := nrcmr_rename_for_cloudant (List.map fst env_vars) e_mr in
     e_mr.
 
-  Definition nrcmr_to_cldmr_chain_translate (h:list (string*string)) (env_vars:list (var * localization)) (e_mr:nrcmr) : cld_mrl :=
+  Definition nrcmr_to_cldmr_chain_translate (h:list (string*string)) (env_vars:list (var * dlocalization)) (e_mr:nrcmr) : cld_mrl :=
     NNRCMRtoNNRCMRCloudantTop h env_vars e_mr.
 
-  Definition nrcmr_to_cldmr_chain_with_prepare (h:list (string*string)) (env_vars:list (var * localization)) (e_mr:nrcmr) : cld_mrl :=
+  Definition nrcmr_to_cldmr_chain_with_prepare (h:list (string*string)) (env_vars:list (var * dlocalization)) (e_mr:nrcmr) : cld_mrl :=
     let e_mr := nrcmr_to_nrcmr_prepared_for_cldmr env_vars e_mr in
     let cld_mr := NNRCMRtoNNRCMRCloudantTop h env_vars e_mr in
     cld_mr.
@@ -72,7 +71,7 @@ Module CompBack(runtime:CompilerRuntime).
   (* To Cloudant *)
 
   Definition nrcmr_to_cloudant_code_gen_with_prepare
-             (h:list (string*string)) (env_vars:list (var * localization)) (e_mr:nrcmr) (rulename:string) : (list (string*string) * (string * list string)) :=
+             (h:list (string*string)) (env_vars:list (var * dlocalization)) (e_mr:nrcmr) (rulename:string) : (list (string*string) * (string * list string)) :=
     let mrl := nrcmr_to_cldmr_chain_with_prepare h env_vars e_mr in
     mapReducePairstoCloudant h mrl rulename.
 
@@ -83,19 +82,19 @@ Module CompBack(runtime:CompilerRuntime).
 
   Require Import NNRCMRtoSpark ForeignToSpark.
 
-  Definition nrcmr_to_nrcmr_prepared_for_spark (env_vars:list (var * localization)) (e_mr:nrcmr) : nrcmr :=
+  Definition nrcmr_to_nrcmr_prepared_for_spark (env_vars:list (var * dlocalization)) (e_mr:nrcmr) : nrcmr :=
     let e_mr := foreign_to_spark_prepare_nrcmr e_mr in
     let e_mr := mr_optimize e_mr in
     let e_mr := foreign_to_spark_prepare_nrcmr e_mr in
     let e_mr := nrcmr_rename_for_spark (List.map fst env_vars) e_mr in
     e_mr.
 
-  Definition mrchain_to_spark_code_gen_with_prepare rulename (env_vars:list (var * localization)) (e_mr:nrcmr) :=
+  Definition mrchain_to_spark_code_gen_with_prepare rulename (env_vars:list (var * dlocalization)) (e_mr:nrcmr) :=
     let e_mr := nrcmr_to_nrcmr_prepared_for_spark env_vars e_mr in
     let spark_mr := nrcmrToSparkTopDataFromFileTop rulename init_vinit env_vars e_mr in
     spark_mr.
 
-  Definition mrchain_to_spark_code_gen rulename (env_vars:list (var * localization)) (e_mr:nrcmr) :=
+  Definition mrchain_to_spark_code_gen rulename (env_vars:list (var * dlocalization)) (e_mr:nrcmr) :=
     nrcmrToSparkTopDataFromFileTop rulename init_vinit env_vars e_mr.
 
 End CompBack.
